Native support for bitfields, first stage
In CompCert C and Clight, this commit adds a "bitfield" designator to l-value expressions and to the results of their evaluation.

Bitfield designators are either
- `Full`: no bit field, the value accessed is that contained in memory at the given block and offset
- `Bits carrier pos width`: the value accessed is `width` bits starting at bit position `pos` in the integer of size `carrier` contained in memory at the given block and offset.

During Csharpminor generation, bitfield accesses are implemented by integer shifts and masks.

Currently, all l-value expressions produce a `Full` bitfield, so the `Bits` case is never exercised.  This will change next when the layout algorithm for struct members is extended to deal with bitfield members.

cfrontend/PrintCsyntax.ml
@@ -204,7 +204,7 @@ let rec expr p (prec, e) =
   then fprintf p "@[<hov 2>("
   else fprintf p "@[<hov 2>";
   begin match e with
-  | Eloc(b, ofs, _) ->
+  | Eloc(b, ofs, _, _) ->
       fprintf p "<loc%a>" !print_pointer_hook (b, ofs)
   | Evar(id, _) ->
       fprintf p "%s" (extern_atom id)
