cfrontend/Cop.v
@@ -1084,6 +1084,44 @@ Definition incrdecr_type (ty: type) :=
   | _ => Tvoid
   end.
 
+(** ** Accessing bit fields *)
+
+Definition chunk_for_carrier (sz: intsize) : memory_chunk :=
+  match sz with
+  | I8 | IBool => Mint8unsigned
+  | I16 => Mint16unsigned
+  | I32 => Mint32
+  end.
+
+Definition bitsize_intsize (sz: intsize) : Z :=
+  match sz with
+  | I8 => 8
+  | I16 => 16
+  | I32 => 32
+  | IBool => 1
+  end.
+
+Definition bitfield_extract (sz: intsize) (sg: signedness) (pos width: Z) (c: int) : int :=
+  if intsize_eq sz IBool || signedness_eq sg Unsigned
+  then Int.unsigned_bitfield_extract pos width c
+  else Int.signed_bitfield_extract pos width c.
+
+Inductive load_bitfield: type -> intsize -> Z -> Z -> mem -> val -> val -> Prop :=
+  | load_bitfield_intro: forall sz sg attr carrier pos width m addr c,
+      0 <= pos -> 0 < width -> pos + width <= Int.zwordsize ->
+      width <= bitsize_intsize sz ->
+      Mem.loadv (chunk_for_carrier carrier) m addr = Some (Vint c) ->
+      load_bitfield (Tint sz sg attr) carrier pos width m addr
+                    (Vint (bitfield_extract sz sg pos width c)).
+
+Inductive store_bitfield: type -> intsize -> Z -> Z -> mem -> val -> val -> mem -> Prop :=
+  | store_bitfield_intro: forall sz sg attr carrier pos width m addr c n m',
+      0 <= pos -> 0 < width -> pos + width <= Int.zwordsize ->
+      width <= bitsize_intsize sz ->
+      Mem.loadv (chunk_for_carrier carrier) m addr = Some (Vint c) ->
+      Mem.storev (chunk_for_carrier carrier) m addr (Vint (Int.bitfield_insert pos width c n)) = Some m' ->
+      store_bitfield (Tint sz sg attr) carrier pos width m addr (Vint n) m'.
+
 (** * Compatibility with extensions and injections *)
 
 Section GENERIC_INJECTION.
