cfrontend/Ctyping.v
@@ -410,8 +410,8 @@ Inductive wt_rvalue : expr -> Prop :=
       wt_rvalue (Eparen r tycast ty)
 
 with wt_lvalue : expr -> Prop :=
-  | wt_Eloc: forall b ofs ty,
-      wt_lvalue (Eloc b ofs ty)
+  | wt_Eloc: forall b ofs bf ty,
+      wt_lvalue (Eloc b ofs bf ty)
   | wt_Evar: forall x ty,
       e!x = Some ty ->
       wt_lvalue (Evar x ty)
@@ -440,7 +440,7 @@ Definition wt_expr_kind (k: kind) (a: expr) :=
 
 Definition expr_kind (a: expr) : kind :=
   match a with
-  | Eloc _ _ _ => LV
+  | Eloc _ _ _ _ => LV
   | Evar _ _ => LV
   | Ederef _ _ => LV
   | Efield _ _ _ => LV
@@ -596,7 +596,7 @@ Fixpoint check_arguments (el: exprlist) (tyl: typelist) : res unit :=
 
 Definition check_rval (e: expr) : res unit :=
   match e with
-  | Eloc _ _ _ | Evar _ _ | Ederef _ _ | Efield _ _ _ =>
+  | Eloc _ _ _ _ | Evar _ _ | Ederef _ _ | Efield _ _ _ =>
       Error (msg "not a r-value")
   | _ =>
       OK tt
@@ -604,7 +604,7 @@ Definition check_rval (e: expr) : res unit :=
 
 Definition check_lval (e: expr) : res unit :=
   match e with
-  | Eloc _ _ _ | Evar _ _ | Ederef _ _ | Efield _ _ _ =>
+  | Eloc _ _ _ _ | Evar _ _ | Ederef _ _ | Efield _ _ _ =>
       OK tt
   | _ =>
       Error (msg "not a l-value")
@@ -846,7 +846,7 @@ Fixpoint retype_expr (ce: composite_env) (e: typenv) (a: expr) : res expr :=
       do r1' <- retype_expr ce e r1; do rl' <- retype_exprlist ce e rl; ecall r1' rl'
   | Ebuiltin ef tyargs rl tyres =>
       do rl' <- retype_exprlist ce e rl; ebuiltin ef tyargs rl' tyres
-  | Eloc _ _ _ =>
+  | Eloc _ _ _ _ =>
       Error (msg "Eloc in source")
   | Eparen _ _ _ =>
       Error (msg "Eparen in source")
@@ -1657,8 +1657,8 @@ Proof.
 Qed.
 
 Lemma wt_deref_loc:
-  forall ge ty m b ofs t v,
-  deref_loc ge ty m b ofs t v ->
+  forall ge ty m b ofs bf t v,
+  deref_loc ge ty m b ofs bf t v ->
   wt_val v ty.
 Proof.
   induction 1.
@@ -1680,6 +1680,12 @@ Proof.
   destruct ty; simpl in H; try discriminate; auto with ty.
   destruct i; destruct s; discriminate.
   destruct f; discriminate.
+- (* bitfield *)
+  inv H0. constructor.
+  destruct sz; cbn in *; auto.
+  + destruct sg; cbn. apply Int.sign_ext_widen; lia. apply Int.zero_ext_widen; lia.
+  + destruct sg; cbn. apply Int.sign_ext_widen; lia. apply Int.zero_ext_widen; lia.
+  + apply Int.zero_ext_widen; lia.
 Qed.
 
 Lemma wt_cast_self:
